# baseURI: https://w3id.org/bcom
# prefix: bcom

@prefix bcom: <https://w3id.org/bcom#> .
@prefix cc: <http://creativecommons.org/ns#> .
@prefix dc: <http://purl.org/dc/terms/> .
@prefix foaf: <http://xmlns.com/foaf/0.1/> .
@prefix owl: <http://www.w3.org/2002/07/owl#> .
@prefix rdf: <http://www.w3.org/1999/02/22-rdf-syntax-ns#> .
@prefix rdfs: <http://www.w3.org/2000/01/rdf-schema#> .
@prefix vann: <http://purl.org/vocab/vann/> .
@prefix vcard: <http://www.w3.org/2006/vcard/ns#> .
@prefix vs: <http://www.w3.org/2003/06/sw-vocab-status/ns#> .
@prefix xsd: <http://www.w3.org/2001/XMLSchema#> .

<https://w3id.org/bcom>
  rdf:type owl:Ontology ;
  dc:created "2021-01-20"^^xsd:date ;
  dc:creator [
      rdf:type foaf:Person ;
      foaf:name "Liu Liu, Ruhr University Bochum" ;
    ] ;
  dc:creator [
      rdf:type foaf:Person ;
      foaf:name "Philipp Hagedorn, Ruhr University Bochum" ;
    ] ;
  dc:description "The Building Concrete Monitoring Ontology (BCOM) is defined for capturing information of concrete work, concrete curing and testing of concrete properties. Further Information on the development and usage of the Ontology can be found in the following publication: Liu et al. (2021): An ontology integrating as-built information for infrastructure asset management using BIM and semantic web. In: Proceedings of 2021 European Conference on Computing in Construction, Online eConference, URL: https://ec-3.org/publications/conferences/2021/paper/?id=167"@en ;
  dc:issued "2021-01-20"^^xsd:date ;
  dc:license "https://creativecommons.org/licenses/by/4.0/"^^xsd:anyURI ;
  dc:modified "2021-07-21"^^xsd:date ;
  dc:publisher [
      rdf:type foaf:Organization ;
      foaf:name "Chair of Computing in Engineering, Ruhr University Bochum" ;
    ] ;
  dc:bibliographicCitation <https://ec-3.org/publications/conferences/2021/paper/?id=167>;
  dc:rights "Copyright 2021 by Chair of Computing in Engineering, Ruhr University Bochum" ;
  dc:source "https://github.com/RUB-Informatik-im-Bauwesen/bcom"^^xsd:anyURI ;
  dc:title "Building Concrete Monitoring Ontology (BCOM)"@en ;
  vann:preferredNamespacePrefix "bcom" ;
  vann:preferredNamespaceUri "https://w3id.org/bcom" ;
  rdfs:comment "-Version 0.3: with additional metadata -Version 0.2: added/changed relations between classes -Version 0.1: initial version of ontology"@en ;
  owl:versionIRI "https://w3id.org/bcom"^^xsd:anyURI ;
  owl:versionInfo "0.3" ;
.
bcom:AirTemperature
  rdf:type owl:DatatypeProperty ;
  rdfs:comment "air temperature during concreting or testing on fresh concrete in degree Celsius"@en ;
  rdfs:domain [
      rdf:type owl:Class ;
      owl:unionOf (
          bcom:ConcretePlacement
          bcom:TestSample
        ) ;
    ] ;
  rdfs:isDefinedBy bcom: ;
  rdfs:label "air temperature"@en ;
  rdfs:range xsd:decimal ;
  vs:term_status "stable" ;
.
bcom:BeginDate
  rdf:type owl:DatatypeProperty ;
  rdfs:comment "begin date of concrete curing with format year-month-day in yyyy-mm-dd"@en ;
  rdfs:domain bcom:ConcreteCuring ;
  rdfs:isDefinedBy bcom: ;
  rdfs:label "begin date"@en ;
  rdfs:range xsd:date ;
  vs:term_status "stable" ;
.
bcom:BeginTimeOfPlacement
  rdf:type owl:DatatypeProperty ;
  rdfs:comment "begin time of concrete placement with format hour-minute-second in hh:mm:ss"@en ;
  rdfs:domain bcom:ConcreteDelivery ;
  rdfs:isDefinedBy bcom: ;
  rdfs:label "begin time"@en ;
  rdfs:range xsd:time ;
  vs:term_status "stable" ;
.
bcom:BulkDensity
  rdf:type owl:DatatypeProperty ;
  rdfs:comment "bulk density of fresh concrete in kg/m^3"@en ;
  rdfs:domain bcom:FreshConcreteProperties ;
  rdfs:isDefinedBy bcom: ;
  rdfs:label "bulk density"@en ;
  rdfs:range xsd:decimal ;
  vs:term_status "stable" ;
.
bcom:ClassOfMonitoring
  rdf:type owl:DatatypeProperty ;
  rdfs:comment "class of concrete monitoring according to DIN EN 13670 / DIN 1045-3 related to the properties of hardened concrete"@en ;
  rdfs:domain bcom:ConcretePlacement ;
  rdfs:isDefinedBy bcom: ;
  rdfs:label "class of monitoring"@en ;
  rdfs:range [
      rdf:type rdfs:Datatype ;
      owl:oneOf (
          "Class 1"
          "Class 2"
          "Class 3"
        ) ;
    ] ;
  vs:term_status "stable" ;
.
bcom:ConcreteCuring
  rdf:type owl:Class ;
  rdfs:comment "This class provides information about the curing process after a concrete placement."@en ;
  rdfs:isDefinedBy bcom: ;
  rdfs:label "Concrete curing"@en ;
  rdfs:subClassOf owl:Thing ;
  vs:term_status "stable" ;
.
bcom:ConcreteDelivery
  rdf:type owl:Class ;
  rdfs:comment "This class provides information about a concrete delivery."@en ;
  rdfs:isDefinedBy bcom: ;
  rdfs:label "Concrete delivery"@en ;
  rdfs:subClassOf owl:Thing ;
  vs:term_status "stable" ;
.
bcom:ConcretePlacement
  rdf:type owl:Class ;
  rdfs:comment "This class provides information about a concreting process itself."@en ;
  rdfs:isDefinedBy bcom: ;
  rdfs:label "Concrete placement"@en ;
  rdfs:subClassOf owl:Thing ;
  vs:term_status "stable" ;
.
bcom:ConcreteTemperature
  rdf:type owl:DatatypeProperty ;
  rdfs:comment "fresh concrete temperature during testing of properties in degree Celsius"@en ;
  rdfs:domain bcom:FreshConcreteProperties ;
  rdfs:isDefinedBy bcom: ;
  rdfs:label "fresh concrete temperature"@en ;
  rdfs:range xsd:decimal ;
  vs:term_status "stable" ;
.
bcom:Condition
  rdf:type owl:DatatypeProperty ;
  rdfs:comment "description of storage conditions"@en ;
  rdfs:domain bcom:Storage ;
  rdfs:isDefinedBy bcom: ;
  rdfs:label "storage condition"@en ;
  rdfs:range xsd:string ;
  vs:term_status "stable" ;
.
bcom:ConformityOfCompressiveStrength
  rdf:type owl:Class ;
  rdfs:comment "This class provides information needed for performing and evaluating the conformity of concrete compressive strength."@en ;
  rdfs:isDefinedBy bcom: ;
  rdfs:label "Conformity testing of compressive strength"@en ;
  rdfs:subClassOf bcom:Test ;
  vs:term_status "stable" ;
.
bcom:ConversionFactor
  rdf:type owl:DatatypeProperty ;
  rdfs:comment "conversion factor of compressive strength testing"@en ;
  rdfs:domain bcom:ConformityOfCompressiveStrength ;
  rdfs:isDefinedBy bcom: ;
  rdfs:label "conversion factor"@en ;
  rdfs:range xsd:decimal ;
  vs:term_status "stable" ;
.
bcom:DateOfConcreting
  rdf:type owl:DatatypeProperty ;
  rdfs:comment "date of concreting with format year-month-day in yyyy-mm-dd"@en ;
  rdfs:domain bcom:ConcretePlacement ;
  rdfs:isDefinedBy bcom: ;
  rdfs:label "date of concreting"@en ;
  rdfs:range xsd:date ;
  vs:term_status "stable" ;
.
bcom:DateOfStripping
  rdf:type owl:DatatypeProperty ;
  rdfs:comment "date of stripping with format year-month-day in yyyy-mm-dd"@en ;
  rdfs:domain bcom:ConcretePlacement ;
  rdfs:isDefinedBy bcom: ;
  rdfs:label "date of stripping"@en ;
  rdfs:range xsd:date ;
  vs:term_status "stable" ;
.
bcom:DeliversConcreteFor
  rdf:type owl:ObjectProperty ;
  rdfs:comment "This property links a concrete delivery to its concrete placement activity where it was used for."@en ;
  rdfs:domain bcom:ConcreteDelivery ;
  rdfs:isDefinedBy bcom: ;
  rdfs:label "delivers concrete for"@en ;
  rdfs:range bcom:ConcretePlacement ;
  rdfs:subClassOf owl:TopObjectProperty ;
  owl:inverseOf bcom:HasDelivery ;
  vs:term_status "stable" ;
.
bcom:DeliveryNote
  rdf:type owl:DatatypeProperty ;
  rdfs:comment "delivery note of mixed-ready concrete"@en ;
  rdfs:domain bcom:ConcreteDelivery ;
  rdfs:isDefinedBy bcom: ;
  rdfs:label "delivery note"@en ;
  rdfs:range xsd:anyURI ;
  vs:term_status "stable" ;
.
bcom:Duration
  rdf:type owl:DatatypeProperty ;
  rdfs:comment "duration of  storage for test sample in days"@en ;
  rdfs:domain bcom:Storage ;
  rdfs:isDefinedBy bcom: ;
  rdfs:label "duration"@en ;
  rdfs:range xsd:decimal ;
  vs:term_status "stable" ;
.
bcom:EndDate
  rdf:type owl:DatatypeProperty ;
  rdfs:comment "end date of concrete curing with format year-month-day in yyyy-mm-dd"@en ;
  rdfs:domain bcom:ConcreteCuring ;
  rdfs:isDefinedBy bcom: ;
  rdfs:label "end date"@en ;
  rdfs:range xsd:date ;
  vs:term_status "stable" ;
.
bcom:EndTimeOfPlacement
  rdf:type owl:DatatypeProperty ;
  rdfs:comment "end time of concrete placement with format hour-minute-second in hh:mm:ss"@en ;
  rdfs:domain bcom:ConcreteDelivery ;
  rdfs:isDefinedBy bcom: ;
  rdfs:label "end time of placement"@en ;
  rdfs:range xsd:time ;
  vs:term_status "stable" ;
.
bcom:EvaluationOfTest
  rdf:type owl:DatatypeProperty ;
  rdfs:comment "evaluation of the mean value of the test in N/mm^2"@en ;
  rdfs:domain bcom:ConformityOfCompressiveStrength ;
  rdfs:isDefinedBy bcom: ;
  rdfs:label "evaluation of test"@en ;
  rdfs:range xsd:decimal ;
  vs:term_status "stable" ;
.
bcom:FinalCompressiveStrength
  rdf:type owl:DatatypeProperty ;
  rdfs:comment "result of the compressive strength of the respective test sample under consideration of the conversion factor in N/mm^2"@en ;
  rdfs:domain bcom:ConformityOfCompressiveStrength ;
  rdfs:isDefinedBy bcom: ;
  rdfs:label "final compressive strength"@en ;
  rdfs:range xsd:decimal ;
  vs:term_status "stable" ;
.
bcom:FreshConcreteProperties
  rdf:type owl:Class ;
  rdfs:comment "This class represents a group of fresh concrete properties.  A fresh concrete propertyset object will usually contain density, voids ratio, consistency."@en ;
  rdfs:isDefinedBy bcom: ;
  rdfs:label "Fresh concrete properties"@en ;
  rdfs:subClassOf bcom:Test ;
  vs:term_status "stable" ;
.
bcom:FreshConcreteTemperature
  rdf:type owl:DatatypeProperty ;
  rdfs:comment "fresh concrete temperature before concrete placement in degree Celsius"@en ;
  rdfs:domain bcom:ConcretePlacement ;
  rdfs:isDefinedBy bcom: ;
  rdfs:label "fresh concrete temperature"@en ;
  rdfs:range xsd:decimal ;
  vs:term_status "stable" ;
.
bcom:HasConcretePlacement
  rdf:type owl:ObjectProperty ;
  rdfs:comment "This property links a concrete curing process to its concrete placement activity."@en ;
  rdfs:domain bcom:ConcreteCuring ;
  rdfs:isDefinedBy bcom: ;
  rdfs:label "has concrete placement"@en ;
  rdfs:range bcom:ConcretePlacement ;
  rdfs:subClassOf owl:TopObjectProperty ;
  owl:inverseOf bcom:HasCuring ;
  vs:term_status "stable" ;
.
bcom:HasCuring
  rdf:type owl:ObjectProperty ;
  rdfs:comment "This property links a concrete placement activity to its curing process."@en ;
  rdfs:domain bcom:ConcretePlacement ;
  rdfs:isDefinedBy bcom: ;
  rdfs:label "has curing"@en ;
  rdfs:range bcom:ConcreteCuring ;
  owl:inverseOf bcom:HasConcretePlacement ;
  vs:term_status "stable" ;
.
bcom:HasDelivery
  rdf:type owl:ObjectProperty ;
  rdfs:comment "This property links a concrete placement activity to its concrete delivery providing the used concrete."@en ;
  rdfs:domain bcom:ConcretePlacement ;
  rdfs:isDefinedBy bcom: ;
  rdfs:label "has delivery"@en ;
  rdfs:range bcom:ConcreteDelivery ;
  owl:inverseOf bcom:SuppliesConcreteTo ;
  vs:term_status "stable" ;
.
bcom:HasStorage
  rdf:type owl:ObjectProperty ;
  rdfs:comment "This property links a concrete test sample to its storage details."@en ;
  rdfs:domain bcom:TestSample ;
  rdfs:isDefinedBy bcom: ;
  rdfs:label "has storage"@en ;
  rdfs:range bcom:Storage ;
  owl:inverseOf bcom:StoresSample ;
  vs:term_status "stable" ;
.
bcom:HasSupplier
  rdf:type owl:ObjectProperty ;
  rdfs:comment "This property links a concrete delivery to its supplier."@en ;
  rdfs:domain bcom:ConcreteDelivery ;
  rdfs:isDefinedBy bcom: ;
  rdfs:label "has supplier"@en ;
  rdfs:range vcard:Organization ;
  owl:inverseOf bcom:SuppliesConcreteTo ;
  vs:term_status "stable" ;
.
bcom:HasTest
  rdf:type owl:ObjectProperty ;
  rdfs:comment "This property links a concrete placement activity to its test procedure."@en ;
  rdfs:domain bcom:ConcretePlacement ;
  rdfs:isDefinedBy bcom: ;
  rdfs:label "has test"@en ;
  rdfs:range bcom:Test ;
  owl:inverseOf bcom:IsTestOf ;
  vs:term_status "stable" ;
.
bcom:HasTestOrganisation
  rdf:type owl:ObjectProperty ;
  rdfs:comment "This property links a test procedure to its organization which is performing the test."@en ;
  rdfs:domain bcom:Test ;
  rdfs:isDefinedBy bcom: ;
  rdfs:label "has test organisation"@en ;
  rdfs:range vcard:Organization ;
  owl:inverseOf bcom:IsTestOrganisationOf ;
  vs:term_status "stable" ;
.
bcom:HasTestPerson
  rdf:type owl:ObjectProperty ;
  rdfs:comment "This property links a test procedure to its person who is performing the test."@en ;
  rdfs:domain bcom:Test ;
  rdfs:isDefinedBy bcom: ;
  rdfs:label "has test person"@en ;
  rdfs:range vcard:Individual ;
  owl:inverseOf bcom:IsTestPersonOf ;
  vs:term_status "stable" ;
.
bcom:HasTestSample
  rdf:type owl:ObjectProperty ;
  rdfs:comment "This property links a test procedure to its test samples tested within this procedure."@en ;
  rdfs:domain bcom:Test ;
  rdfs:isDefinedBy bcom: ;
  rdfs:label "has test sample"@en ;
  rdfs:range bcom:TestSample ;
  owl:inverseOf bcom:IsTestSampleOf ;
  vs:term_status "stable" ;
.
bcom:Height
  rdf:type owl:DatatypeProperty ;
  rdfs:comment "height of a test sample as cube or as cylinder in mm"@en ;
  rdfs:domain bcom:TestSample ;
  rdfs:isDefinedBy bcom: ;
  rdfs:label "height"@en ;
  rdfs:range xsd:decimal ;
  vs:term_status "stable" ;
.
bcom:Humidity
  rdf:type owl:DatatypeProperty ;
  rdfs:comment "relative humidity of storage condition in %"@en ;
  rdfs:domain bcom:Storage ;
  rdfs:isDefinedBy bcom: ;
  rdfs:label "humidity"@en ;
  rdfs:range xsd:decimal ;
  vs:term_status "stable" ;
.
bcom:InterimCompressiveStrength
  rdf:type owl:DatatypeProperty ;
  rdfs:comment "intermediate result of the compressive strength of the respective sample without conversion factor of in N/mm^2"@en ;
  rdfs:domain bcom:ConformityOfCompressiveStrength ;
  rdfs:isDefinedBy bcom: ;
  rdfs:label "intermediate compressive strength"@en ;
  rdfs:range xsd:decimal ;
  vs:term_status "stable" ;
.
bcom:IsTestOf
  rdf:type owl:ObjectProperty ;
  rdfs:comment "This property links a test procedure to its concrete placement activity whithin its test samples have been concreted."@en ;
  rdfs:domain bcom:Test ;
  rdfs:isDefinedBy bcom: ;
  rdfs:label "is test of"@en ;
  rdfs:range bcom:ConcretePlacement ;
  owl:inverseOf bcom:HasTest ;
  vs:term_status "stable" ;
.
bcom:IsTestOrganisationOf
  rdf:type owl:ObjectProperty ;
  rdfs:comment "This property links an organization to its test procedures that have been performed by itself."@en ;
  rdfs:domain vcard:Organization ;
  rdfs:isDefinedBy bcom: ;
  rdfs:label "is test organisation of"@en ;
  rdfs:range bcom:Test ;
  rdfs:subClassOf owl:TopObjectProperty ;
  owl:inverseOf bcom:HasTestOrganisation ;
  vs:term_status "stable" ;
.
bcom:IsTestPersonOf
  rdf:type owl:ObjectProperty ;
  rdfs:comment "This property links a test examining person to its test procedures that have been performed by itslef."@en ;
  rdfs:domain vcard:Individual ;
  rdfs:isDefinedBy bcom: ;
  rdfs:label "is test person of" ;
  rdfs:range bcom:Test ;
  owl:inverseOf bcom:HasTestPerson ;
  vs:term_status "stable" ;
.
bcom:IsTestSampleOf
  rdf:type owl:ObjectProperty ;
  rdfs:comment "This property links a test sample to its test procedure within which it has been tested."@en ;
  rdfs:domain bcom:TestSample ;
  rdfs:isDefinedBy bcom: ;
  rdfs:label "is test sample of"@en ;
  rdfs:range bcom:Test ;
  owl:inverseOf bcom:HasTestSample ;
  vs:term_status "stable" ;
.
bcom:Length
  rdf:type owl:DatatypeProperty ;
  rdfs:comment "length of a test sample for cubes in mm"@en ;
  rdfs:domain bcom:TestSample ;
  rdfs:isDefinedBy bcom: ;
  rdfs:label "length"@en ;
  rdfs:range xsd:decimal ;
  vs:term_status "stable" ;
.
bcom:MaturityOfConcrete
  rdf:type owl:DatatypeProperty ;
  rdfs:comment "maturity of concrete in minutes"@en ;
  rdfs:domain bcom:FreshConcreteProperties ;
  rdfs:isDefinedBy bcom: ;
  rdfs:label "maturity of concrete"@en ;
  rdfs:range xsd:decimal ;
  vs:term_status "stable" ;
.
bcom:MaxAirTemperature
  rdf:type owl:DatatypeProperty ;
  rdfs:comment "maximum air temperature during post-treatment in degree Celsius"@en ;
  rdfs:domain bcom:ConcreteCuring ;
  rdfs:isDefinedBy bcom: ;
  rdfs:label "max air temperature"@en ;
  rdfs:range xsd:decimal ;
  vs:term_status "stable" ;
.
bcom:MethodOfAftertreatment
  rdf:type owl:DatatypeProperty ;
  rdfs:comment "description for the method of concrete curing"@en ;
  rdfs:domain bcom:ConcreteCuring ;
  rdfs:isDefinedBy bcom: ;
  rdfs:label "method of aftertreatment"@en ;
  rdfs:range xsd:string ;
  vs:term_status "stable" ;
.
bcom:MinAirTemperature
  rdf:type owl:DatatypeProperty ;
  rdfs:comment "minimum air temperature during post-treatment in degree Celsius"@en ;
  rdfs:domain bcom:ConcreteCuring ;
  rdfs:isDefinedBy bcom: ;
  rdfs:label "min air temperature"@en ;
  rdfs:range xsd:decimal ;
  vs:term_status "stable" ;
.
bcom:NormativeReference
  rdf:type owl:DatatypeProperty ;
  rdfs:comment "norm or standard of the test method"@en ;
  rdfs:domain bcom:ConformityOfCompressiveStrength ;
  rdfs:isDefinedBy bcom: ;
  rdfs:label "normative reference"@en ;
  rdfs:range xsd:string ;
  vs:term_status "stable" ;
.
bcom:ObjectTemperature
  rdf:type owl:DatatypeProperty ;
  rdfs:comment "object temperature of a test sample in degree Celsius"@en ;
  rdfs:domain bcom:TestSample ;
  rdfs:isDefinedBy bcom: ;
  rdfs:label "object temperature"@en ;
  rdfs:range xsd:decimal ;
  vs:term_status "stable" ;
.
bcom:QuantityOfConcrete
  rdf:type owl:DatatypeProperty ;
  rdfs:comment "quantity of the concrete placement in cubature m^3"@en ;
  rdfs:domain bcom:ConcretePlacement ;
  rdfs:isDefinedBy bcom: ;
  rdfs:label "quantity of concrete"@en ;
  rdfs:range xsd:decimal ;
  vs:term_status "stable" ;
.
bcom:RateOfFlowTableTest
  rdf:type owl:DatatypeProperty ;
  rdfs:comment "rate of flow table test according to DIN EN 12350-5 in mm"@en ;
  rdfs:domain bcom:FreshConcreteProperties ;
  rdfs:isDefinedBy bcom: ;
  rdfs:label "rate of flow table test"@en ;
  rdfs:range xsd:decimal ;
  vs:term_status "stable" ;
.
bcom:SampleID
  rdf:type owl:DatatypeProperty ;
  rdfs:comment "name or ID of the test sample"@en ;
  rdfs:domain bcom:TestSample ;
  rdfs:isDefinedBy bcom: ;
  rdfs:label "sample ID"@en ;
  rdfs:range xsd:string ;
  vs:term_status "stable" ;
.
bcom:SamplingDate
  rdf:type owl:DatatypeProperty ;
  rdfs:comment "date of sampling with format year-month-day in yyyy-mm-dd"@en ;
  rdfs:domain bcom:TestSample ;
  rdfs:isDefinedBy bcom: ;
  rdfs:label "sampling date"@en ;
  rdfs:range xsd:date ;
  vs:term_status "stable" ;
.
bcom:Storage
  rdf:type owl:Class ;
  rdfs:comment "This class represents the storage conditions of a test sample."@en ;
  rdfs:isDefinedBy bcom: ;
  rdfs:label "Storage"@en ;
  rdfs:subClassOf owl:Thing ;
  vs:term_status "stable" ;
.
bcom:StoresSample
  rdf:type owl:ObjectProperty ;
  rdfs:comment "This property links storage details to its test samples that has been stored under the specific storage conditions."@en ;
  rdfs:domain bcom:Storage ;
  rdfs:isDefinedBy bcom: ;
  rdfs:label "stores sample"@en ;
  rdfs:range bcom:TestSample ;
  owl:inverseOf bcom:HasStorage ;
  vs:term_status "stable" ;
.
bcom:SuppliesConcreteTo
  rdf:type owl:ObjectProperty ;
  rdfs:comment "This property links an organization to its concrete placement activities where it delivered concrete for."@en ;
  rdfs:domain vcard:Organization ;
  rdfs:isDefinedBy bcom: ;
  rdfs:label "supplies concrete to"@en ;
  rdfs:range bcom:ConcretePlacement ;
  rdfs:subClassOf owl:TopObjectProperty ;
  owl:inverseOf bcom:HasSupplier ;
  vs:term_status "stable" ;
.
bcom:Temperature
  rdf:type owl:DatatypeProperty ;
  rdfs:comment "storage temperature in degree Celsius"@en ;
  rdfs:domain bcom:Storage ;
  rdfs:isDefinedBy bcom: ;
  rdfs:label "temperature"@en ;
  rdfs:range xsd:decimal ;
  vs:term_status "stable" ;
.
bcom:Test
  rdf:type owl:Class ;
  rdfs:comment "This class represents the super-class for different types of tests, that can be performed on placed concrete."@en ;
  rdfs:isDefinedBy bcom: ;
  rdfs:label "Test"@en ;
  rdfs:subClassOf owl:Thing ;
  vs:term_status "stable" ;
.
bcom:TestCharacteristic
  rdf:type owl:DatatypeProperty ;
  rdfs:comment "the material property that has to be tested"@en ;
  rdfs:domain bcom:ConformityOfCompressiveStrength ;
  rdfs:isDefinedBy bcom: ;
  rdfs:label "tested characteristic"@en ;
  rdfs:range xsd:string ;
  vs:term_status "stable" ;
.
bcom:TestDate
  rdf:type owl:DatatypeProperty ;
  rdfs:comment "date of testing with format year-month-day in yyyy-mm-dd"@en ;
  rdfs:domain bcom:Test ;
  rdfs:isDefinedBy bcom: ;
  rdfs:label "test date"@en ;
  rdfs:range xsd:date ;
  vs:term_status "stable" ;
.
bcom:TestReport
  rdf:type owl:DatatypeProperty ;
  rdfs:comment "report of conformity test of concrete"@en ;
  rdfs:domain bcom:Test ;
  rdfs:isDefinedBy bcom: ;
  rdfs:label "test report"@en ;
  rdfs:range xsd:anyURI ;
  vs:term_status "stable" ;
.
bcom:TestSample
  rdf:type owl:Class ;
  rdfs:comment "This class provides information about test samples."@en ;
  rdfs:isDefinedBy bcom: ;
  rdfs:label "Test sample"@en ;
  rdfs:subClassOf owl:Thing ;
  vs:term_status "stable" ;
.
bcom:TestTime
  rdf:type owl:DatatypeProperty ;
  rdfs:comment "time of testing with format hour-minute-second in hh:mm:ss"@en ;
  rdfs:domain bcom:Test ;
  rdfs:isDefinedBy bcom: ;
  rdfs:label "test time"@en ;
  rdfs:range xsd:time ;
  vs:term_status "stable" ;
.
bcom:TestType
  rdf:type owl:DatatypeProperty ;
  rdfs:comment "type of test as self-inspection or third-party monitoring"@en ;
  rdfs:domain [
      rdf:type owl:Class ;
      owl:unionOf (
          bcom:ConcretePlacement
          bcom:Test
        ) ;
    ] ;
  rdfs:isDefinedBy bcom: ;
  rdfs:label "test type"@en ;
  rdfs:range [
      rdf:type rdfs:Datatype ;
      owl:oneOf (
          "Self-Inspection"
          "Third-Party Monitoring"
        ) ;
    ] ;
  vs:term_status "stable" ;
.
bcom:TestedBreakingLoad
  rdf:type owl:DatatypeProperty ;
  rdfs:comment "value of breaking load of test procedure in N"@en ;
  rdfs:domain bcom:ConformityOfCompressiveStrength ;
  rdfs:isDefinedBy bcom: ;
  rdfs:label "tested breaking load"@en ;
  rdfs:range xsd:decimal ;
  vs:term_status "stable" ;
.
bcom:TestedDensity
  rdf:type owl:DatatypeProperty ;
  rdfs:comment "value of density from a sample in kg/m^3"@en ;
  rdfs:domain bcom:ConformityOfCompressiveStrength ;
  rdfs:isDefinedBy bcom: ;
  rdfs:label "tested density"@en ;
  rdfs:range xsd:decimal ;
  vs:term_status "stable" ;
.
bcom:VoidsRatio
  rdf:type owl:DatatypeProperty ;
  rdfs:comment "voids ratio of fresh concrete in V-%"@en ;
  rdfs:domain bcom:FreshConcreteProperties ;
  rdfs:isDefinedBy bcom: ;
  rdfs:label "voids ratio"@en ;
  rdfs:range xsd:decimal ;
  vs:term_status "stable" ;
.
bcom:Weigth
  rdf:type owl:DatatypeProperty ;
  rdfs:comment "weigth of a test sample in kg"@en ;
  rdfs:domain bcom:TestSample ;
  rdfs:isDefinedBy bcom: ;
  rdfs:label "weigth"@en ;
  rdfs:range xsd:decimal ;
  vs:term_status "stable" ;
.
bcom:WidthOrDia
  rdf:type owl:DatatypeProperty ;
  rdfs:comment "width of a test sample as cube or diameter of a test sample as cylinder in mm"@en ;
  rdfs:domain bcom:TestSample ;
  rdfs:isDefinedBy bcom: ;
  rdfs:label "width or dia"@en ;
  rdfs:range xsd:decimal ;
  vs:term_status "stable" ;
.
